Conform/Main.lean
@@ -5,12 +5,12 @@ def TestsSubdir : System.FilePath := "BlockchainTests"
 def isTestFile (file : System.FilePath) : Bool := file.extension.option false (· == "json")
 
 private def basicSuccess (name : System.FilePath)
-                         (result : Batteries.RBMap String EvmYul.Conform.TestResult compare) : IO Bool := do
+                         (result : Std.TreeMap String EvmYul.Conform.TestResult compare) : IO Bool := do
   if result.all (λ _ v ↦ v.isNone)
   then IO.println s!"SUCCESS! - {name}"; pure true
   else pure false
 
-private def success (result : Batteries.RBMap String EvmYul.Conform.TestResult compare) : Array String × Array String :=
+private def success (result : Std.TreeMap String EvmYul.Conform.TestResult compare) : Array String × Array String :=
   let (succeeded, failed) := result.partition (λ _ v ↦ v.isNone)
   (succeeded.keys, failed.keys)
 
