EvmYul/EVM/Gas.lean
@@ -97,13 +97,13 @@ It would be worth restructing everything to obtain cleaner separation of concern
 -/
 def Csstore (s : EVM.State) : ℕ :=
   let { stack := μₛ, accountMap := σ, σ₀ := σ₀, executionEnv.codeOwner := Iₐ, .. } := s
-  let { storage := σ_Iₐ, .. } := σ.find! Iₐ
+  let { storage := σ_Iₐ, .. } := σ.get! Iₐ
   let storeAddr := μₛ[0]!
   let v₀ :=
-    match σ₀.find? Iₐ with
+    match σ₀.get? Iₐ with
       | none => ⟨0⟩
-      | some acc => acc.storage.findD storeAddr ⟨0⟩
-  let v := σ_Iₐ.findD storeAddr ⟨0⟩
+      | some acc => acc.storage.getD storeAddr ⟨0⟩
+  let v := σ_Iₐ.getD storeAddr ⟨0⟩
   let v' := μₛ[1]!
   let loadComponent :=
     if s.substate.accessedStorageKeys.contains (Iₐ, storeAddr) then
@@ -140,7 +140,7 @@ def Cselfdestruct (s : EVM.State) : ℕ :=
   let { substate.accessedAccounts := Aₐ, accountMap := σ, executionEnv.codeOwner := Iₐ, .. } := s
   let c_cold := if Aₐ.contains r then 0 else Gcoldaccountaccess
   let c_new :=
-    if State.dead σ r ∧ (σ.find? Iₐ |>.option ⟨0⟩ (·.balance)) ≠ ⟨0⟩ then
+    if State.dead σ r ∧ (σ.get? Iₐ |>.option ⟨0⟩ (·.balance)) ≠ ⟨0⟩ then
       Gnewaccount
     else 0
   Gselfdestruct + c_cold + c_new
