EvmYul/EVM/Semantics.lean
@@ -2,6 +2,8 @@ import Mathlib.Data.BitVec
 import Mathlib.Data.Array.Defs
 import Mathlib.Data.Finmap
 import Mathlib.Data.List.Defs
+import Std.Data.TreeSet.Basic
+import Std.Data.TreeMap.AdditionalOperations
 import EvmYul.Data.Stack
 
 import EvmYul.Maps.AccountMap
@@ -33,6 +35,7 @@ import EvmYul.MachineState
 import Conform.Wheels
 
 open EvmYul.DebuggingAndProfiling
+open Std (TreeMap TreeSet)
 
 namespace EvmYul
 
@@ -162,7 +165,7 @@ def call (fuel : Nat)
       let i := evmState.memory.readWithPadding inOffset.toNat inSize.toNat
       let A' := evmState.addAccessedAccount t |>.substate
       let (cA, σ', g', A', z, o) ← do
-        if value ≤ (σ.find? Iₐ |>.option ⟨0⟩ (·.balance)) ∧ Iₑ < 1024 then
+        if value ≤ (σ.get? Iₐ |>.option ⟨0⟩ (·.balance)) ∧ Iₑ < 1024 then
           let resultOfΘ ←
             Θ (fuel := f)
               blobVersionedHashes
@@ -197,7 +200,7 @@ def call (fuel : Nat)
       let μ'_g := μ'ₘ.gasAvailable + g' -- Ccall is subtracted in X as part of C
 
       let codeExecutionFailed   : Bool := !z
-      let notEnoughFunds        : Bool := value > (σ.find? evmState.executionEnv.codeOwner |>.elim ⟨0⟩ (·.balance)) -- TODO - Unify condition with CREATE.
+      let notEnoughFunds        : Bool := value > (σ.get? evmState.executionEnv.codeOwner |>.elim ⟨0⟩ (·.balance)) -- TODO - Unify condition with CREATE.
       let callDepthLimitReached : Bool := evmState.executionEnv.depth == 1024
       let x : UInt256 := if codeExecutionFailed || notEnoughFunds || callDepthLimitReached then ⟨0⟩ else ⟨1⟩ -- where x = 0 if the code execution for this operation failed, or if μs[2] > σ[Ia]b (not enough funds) or Ie = 1024 (call depth limit reached); x = 1 otherwise.
 
@@ -244,14 +247,14 @@ def step (fuel : ℕ) (gasCost : ℕ) (instr : Option (Operation .EVM × Option 
             let Iₒ := evmState.executionEnv.sender
             let Iₑ := evmState.executionEnv.depth
             let σ := evmState.accountMap
-            let σ_Iₐ : Account .EVM := σ.find? Iₐ |>.getD default
+            let σ_Iₐ : Account .EVM := σ.get? Iₐ |>.getD default
             let σStar := σ.insert Iₐ {σ_Iₐ with nonce := σ_Iₐ.nonce + ⟨1⟩}
 
             let (a, evmState', g', z, o)
                   : (AccountAddress × EVM.State × UInt256 × Bool × ByteArray)
               :=
               if σ_Iₐ.nonce.toNat ≥ 2^64-1 then (default, evmState, .ofNat (L evmState.gasAvailable.toNat), False, .empty) else
-              if μ₀ ≤ (σ.find? Iₐ |>.option ⟨0⟩ (·.balance)) ∧ Iₑ < 1024 ∧ i.size ≤ 49152 then
+              if μ₀ ≤ (σ.get? Iₐ |>.option ⟨0⟩ (·.balance)) ∧ Iₑ < 1024 ∧ i.size ≤ 49152 then
                 let Λ :=
                   Lambda f
                     evmState.executionEnv.blobVersionedHashes
@@ -287,7 +290,7 @@ def step (fuel : ℕ) (gasCost : ℕ) (instr : Option (Operation .EVM × Option 
               else
                 (0, evmState, .ofNat (L evmState.gasAvailable.toNat), False, .empty)
             let x : UInt256 :=
-              let balance := σ.find? Iₐ |>.option ⟨0⟩ (·.balance)
+              let balance := σ.get? Iₐ |>.option ⟨0⟩ (·.balance)
                 if z = false ∨ Iₑ = 1024 ∨ μ₀ > balance ∨ i.size > 49152 then ⟨0⟩ else .ofNat a
             let newReturnData : ByteArray := if z then .empty else o
             if (evmState.gasAvailable + g').toNat < L (evmState.gasAvailable.toNat) then
@@ -314,11 +317,11 @@ def step (fuel : ℕ) (gasCost : ℕ) (instr : Option (Operation .EVM × Option 
             let Iₒ := evmState.executionEnv.sender
             let Iₑ := evmState.executionEnv.depth
             let σ := evmState.accountMap
-            let σ_Iₐ : Account .EVM := σ.find? Iₐ |>.getD default
+            let σ_Iₐ : Account .EVM := σ.get? Iₐ |>.getD default
             let σStar := σ.insert Iₐ {σ_Iₐ with nonce := σ_Iₐ.nonce + ⟨1⟩}
             let (a, evmState', g', z, o) : (AccountAddress × EVM.State × UInt256 × Bool × ByteArray) :=
               if σ_Iₐ.nonce.toNat ≥ 2^64-1 then (default, evmState, .ofNat (L evmState.gasAvailable.toNat), False, .empty) else
-              if μ₀ ≤ (σ.find? Iₐ |>.option ⟨0⟩ (·.balance)) ∧ Iₑ < 1024 ∧ i.size ≤ 49152 then
+              if μ₀ ≤ (σ.get? Iₐ |>.option ⟨0⟩ (·.balance)) ∧ Iₑ < 1024 ∧ i.size ≤ 49152 then
                 let Λ :=
                   Lambda f
                     evmState.executionEnv.blobVersionedHashes
@@ -345,7 +348,7 @@ def step (fuel : ℕ) (gasCost : ℕ) (instr : Option (Operation .EVM × Option 
               else
                 (0, evmState, .ofNat (L evmState.gasAvailable.toNat), False, .empty)
             let x : UInt256 :=
-              let balance := σ.find? Iₐ |>.option ⟨0⟩ (·.balance)
+              let balance := σ.get? Iₐ |>.option ⟨0⟩ (·.balance)
                 if z = false ∨ Iₑ = 1024 ∨ μ₀ > balance ∨ i.size > 49152 then ⟨0⟩ else .ofNat a
             let newReturnData : ByteArray := if z then .empty else o
             if (evmState.gasAvailable + g').toNat < L evmState.gasAvailable.toNat then
@@ -524,7 +527,7 @@ def X (fuel : ℕ) (validJumps : Array UInt256) (evmState : State)
 -/
 def Ξ -- Type `Ξ` using `\GX` or `\Xi`
   (fuel : ℕ)
-  (createdAccounts : RBSet AccountAddress compare)
+  (createdAccounts : TreeSet AccountAddress compare)
   (genesisBlockHeader : BlockHeader)
   (blocks : ProcessedBlocks)
   (σ : AccountMap .EVM)
@@ -535,7 +538,7 @@ def Ξ -- Type `Ξ` using `\GX` or `\Xi`
     :
   Except
     EVM.ExecutionException
-    (ExecutionResult (RBSet AccountAddress compare × AccountMap .EVM × UInt256 × Substate))
+    (ExecutionResult (TreeSet AccountAddress compare × AccountMap .EVM × UInt256 × Substate))
 := do
   match fuel with
     | 0 => .error .OutOfFuel
@@ -562,7 +565,7 @@ def Ξ -- Type `Ξ` using `\GX` or `\Xi`
 def Lambda
   (fuel : ℕ)
   (blobVersionedHashes : List ByteArray)
-  (createdAccounts : RBSet AccountAddress compare) -- needed for EIP-6780
+  (createdAccounts : TreeSet AccountAddress compare) -- needed for EIP-6780
   (genesisBlockHeader : BlockHeader)
   (blocks : ProcessedBlocks)
   (σ : AccountMap .EVM)
@@ -581,7 +584,7 @@ def Lambda
   :
   Except EVM.ExecutionException
     ( AccountAddress
-    × RBSet AccountAddress compare
+    × TreeSet AccountAddress compare
     × AccountMap .EVM
     × UInt256
     × Substate
@@ -596,7 +599,7 @@ def Lambda
   -- EIP-3860 (includes EIP-170)
   -- https://eips.ethereum.org/EIPS/eip-3860
 
-  let n : UInt256 := (σ.find? s |>.option ⟨0⟩ (·.nonce)) - ⟨1⟩
+  let n : UInt256 := (σ.get? s |>.option ⟨0⟩ (·.nonce)) - ⟨1⟩
   let lₐ ← L_A s n ζ i
   let a : AccountAddress := -- (94) (95)
     (ffi.KEC lₐ).extract 12 32 /- 160 bits = 20 bytes -/
@@ -605,7 +608,7 @@ def Lambda
   -- A* (97)
   let AStar := A.addAccessedAccount a
   -- σ*
-  let existentAccount := σ.findD a default
+  let existentAccount := σ.getD a default
 
   /-
     https://eips.ethereum.org/EIPS/eip-7610
@@ -632,7 +635,7 @@ def Lambda
 
   -- If `v` ≠ 0 then the sender must have passed the `INSUFFICIENT_ACCOUNT_FUNDS` check
   let σStar :=
-    match σ.find? s with
+    match σ.get? s with
       | none =>  σ
       | some ac =>
         σ.insert s {ac with balance := ac.balance - v}
@@ -663,7 +666,7 @@ def Lambda
 
       let F : Bool := Id.run do -- (118)
         let F₀ : Bool :=
-          match σ.find? a with
+          match σ.get? a with
           | .some ac => ac.code ≠ .empty ∨ ac.nonce ≠ ⟨0⟩
           | .none => false
         let F₂ : Bool := gStarStar.toNat < c
@@ -674,7 +677,7 @@ def Lambda
 
       let σ' : AccountMap .EVM := -- (115)
         if F then σ else
-          let newAccount' := σStarStar.findD a default
+          let newAccount' := σStarStar.getD a default
           σStarStar.insert a {newAccount' with code := returnedData}
 
       -- (114)
@@ -716,7 +719,7 @@ NB - This is implemented using the 'boolean' fragment with ==, <=, ||, etc.
 -/
 def Θ (fuel : Nat)
       (blobVersionedHashes : List ByteArray)
-      (createdAccounts : RBSet AccountAddress compare)
+      (createdAccounts : TreeSet AccountAddress compare)
       (genesisBlockHeader : BlockHeader)
       (blocks : ProcessedBlocks)
       (σ  : AccountMap .EVM)
@@ -735,7 +738,7 @@ def Θ (fuel : Nat)
       (H : BlockHeader)
       (w  : Bool)
         :
-      Except EVM.ExecutionException (RBSet AccountAddress compare × AccountMap .EVM × UInt256 × Substate × Bool × ByteArray)
+      Except EVM.ExecutionException (TreeSet AccountAddress compare × AccountMap .EVM × UInt256 × Substate × Bool × ByteArray)
 :=
   match fuel with
     | 0 => .error .OutOfFuel
@@ -743,7 +746,7 @@ def Θ (fuel : Nat)
 
   -- (124) (125) (126)
   let σ'₁ :=
-    match σ.find? r with
+    match σ.get? r with
       | none =>
         if v != ⟨0⟩ then
           σ.insert r { (default : Account .EVM) with balance := v}
@@ -754,7 +757,7 @@ def Θ (fuel : Nat)
 
   -- If `v` ≠ 0 then the sender must have passed the `INSUFFICIENT_ACCOUNT_FUNDS` check
   let σ₁ :=
-    match σ'₁.find? s with
+    match σ'₁.get? s with
       | none => σ'₁
       | some acc =>
         σ'₁.insert s { acc with balance := acc.balance - v}
@@ -816,9 +819,6 @@ def Θ (fuel : Nat)
 
 end
 
-open Batteries (RBMap RBSet)
-
-
 -- Type Υ using \Upsilon or \GU
 def Υ (fuel : ℕ)
   (σ : AccountMap .EVM)
@@ -832,7 +832,7 @@ def Υ (fuel : ℕ)
 := do
   let g₀ : ℕ := EVM.intrinsicGas T
   -- "here can be no invalid transactions from this point"
-  let senderAccount := (σ.find? S_T).get!
+  let senderAccount := (σ.get? S_T).get!
   -- The priority fee (67)
   let f :=
     match T with
@@ -866,7 +866,7 @@ def Υ (fuel : ℕ)
   let a := -- (80)
     A0.accessedAccounts.insert S_T
       |>.insert H.beneficiary
-      |>.union <| RBSet.ofList (accessList.map Prod.fst) compare
+      |>.union <| TreeSet.ofList (accessList.map Prod.fst) compare
   -- (81)
   let g := .ofNat <| T.base.gasLimit.toNat - g₀
   let AStarₐ := -- (79)
@@ -874,8 +874,8 @@ def Υ (fuel : ℕ)
       | some t => a.insert t
       | none => a
   let AStar := -- (77)
-    { A0 with accessedAccounts := AStarₐ, accessedStorageKeys := RBSet.ofList AStar_K Substate.storageKeysCmp}
-  let createdAccounts : RBSet AccountAddress compare := .empty
+    { A0 with accessedAccounts := AStarₐ, accessedStorageKeys := TreeSet.ofList AStar_K Substate.storageKeysCmp}
+  let createdAccounts : TreeSet AccountAddress compare := .empty
   let (/- provisional state -/ σ_P, g', A, z) ← -- (76)
     match T.base.recipient with
       | none => do
@@ -938,10 +938,10 @@ def Υ (fuel : ℕ)
     if beneficiaryFee != ⟨0⟩ then
       σStar.increaseBalance .EVM H.beneficiary beneficiaryFee
     else σStar
-  let σ' := A.selfDestructSet.1.foldl RBMap.erase σStar' -- (87)
+  let σ' := A.selfDestructSet.foldl (fun acc addr => acc.erase addr) σStar' -- (87)
   let deadAccounts := A.touchedAccounts.filter (State.dead σStar' ·)
-  let σ' := deadAccounts.foldl RBMap.erase σ' -- (88)
-  let σ' := σ'.map λ (addr, acc) ↦ (addr, { acc with tstorage := .empty})
+  let σ' := deadAccounts.foldl (fun acc addr => acc.erase addr) σ' -- (88)
+  let σ' := σ'.map (fun _addr acc => { acc with tstorage := .empty })
   .ok (σ', A, z, T.base.gasLimit - gStar)
 end EVM
 
