EvmYul/Maps/ByteMap.lean
@@ -17,11 +17,8 @@ a'la `Finmap`.
 TODO - All of this is very ugly.
 -/
 
-import Batteries.Data.RBMap.Basic
-import Batteries.Data.RBMap.Depth
-import Batteries.Data.RBMap.Lemmas
-import Batteries.Data.RBMap.Alter
-import Batteries.Data.RBMap.WF
+import Std.Data.TreeMap.Basic
+import Std.Data.TreeMap.Lemmas
 
 import EvmYul.Wheels
 
@@ -29,7 +26,7 @@ namespace EvmYul
 
 section RemoveLater
 
-abbrev ByteMap := Batteries.RBMap UInt256 UInt8 compare
+abbrev ByteMap := Std.TreeMap UInt256 UInt8 compare
 
 end RemoveLater
 
